exercicios_arrays/exercicio4.dfy
@@ -1,15 +1,31 @@
-ghost predicate Sorted(a: array<int>)
+ghost function Product(a: array<int>): int
   reads a
 {
-    //forall j, k :: 0 <= j < k < a.Length ==> a[j] <= a[k]
-    forall i :: 0 <= i < a.Length-1 ==> a[i] <= a[i+1]
+  ProductAux(a, 0, a.Length-1)
 }
 
-method Main()
+ghost function ProductAux(a: array<int>, from: nat, to: int): int
+  requires to < a.Length
+  reads a
 {
-    var a := new int[3];
-    a[0] := 1;
-    a[1] := 3;
-    a[2] := 5;
-    assert Sorted(a);
+  if from > to
+  then 1
+  else if from == to
+       then a[to]
+       else a[to] * ProductAux(a, from, to-1)
+}
+
+method ProductImpl(a: array<int>) returns (p:int)
+  requires a.Length > 0
+  ensures p == Product(a)
+{
+  p := 1;
+  var i := 0;
+  while i < a.Length
+    invariant 0 <= i <= a.Length
+    invariant p == ProductAux(a, 0, i-1)
+  {
+    p := p * a[i];
+    i := i + 1;
+  }
 }
