exercicios_arrays/exercicio2.dfy
@@ -3,18 +3,18 @@ method FindMaxIndex(a:array<int>) returns (i:int)
   ensures 0 <= i < a.Length //é um índice válido
   ensures forall j :: 0 <= j < a.Length ==> a[j] <= a[i] //é o índice do maior elemento
 {
-    var index := 0;
-    i := 0;
-    while index < a.Length
-      invariant 0 <= index <= a.Length
-      invariant 0 <= i < a.Length
-      invariant forall j :: 0 <= j < index ==> a[j] <= a[i]
+  var index := 0;
+  i := 0;
+  while index < a.Length
+    invariant 0 <= index <= a.Length
+    invariant 0 <= i < a.Length
+    invariant forall j :: 0 <= j < index ==> a[j] <= a[i]
     {
-        if a[index] > a[i]
-        {
-            i := index;
-        }
-        index := index + 1;
+      if a[index] > a[i]
+      {
+        i := index;
+      }
+      index := index + 1;
     }
 }
 
