exercicios_arrays/exercicio2b.dfy
@@ -3,18 +3,18 @@ method FindMaxValue(a:array<int>) returns (m:int)
   ensures exists i :: 0 <= i < a.Length && a[i] == m //m é um elemento do array
   ensures forall i :: 0 <= i < a.Length ==> a[i] <= m //m é o maior elemento
 {
-    var index := 0;
-    m := a[index];
-    while index < a.Length
-      invariant 0 <= index <= a.Length
-      invariant forall i :: 0 <= i < index ==> a[i] <= m
-      invariant index == 0 ==> a[0] == m
-      invariant index > 0 ==> exists i :: 0 <= i < index && a[i] == m
+  var index := 0;
+  m := a[index];
+  while index < a.Length
+    invariant 0 <= index <= a.Length
+    invariant forall i :: 0 <= i < index ==> a[i] <= m
+    invariant index == 0 ==> a[0] == m
+    invariant index > 0 ==> exists i :: 0 <= i < index && a[i] == m
     {
-        if a[index] > m
-        {
-            m := a[index];
-        }
-        index := index + 1;
+      if a[index] > m
+      {
+        m := a[index];
+      }
+      index := index + 1;
     }
 }
