exercicios_arrays/exercicio6.dfy
@@ -1,46 +1,14 @@
-ghost predicate sorted(a: array<int>)
-  reads a
+method IncrementaArray(a: array<int>)
+  modifies a
+  ensures forall i :: 0 <= i < a.Length ==> a[i] == old(a[i]) + 1
 {
-    forall j, k :: 0 <= j < k < a.Length ==> a[j] <= a[k]
-}
-
-method BinarySearch(a: array<int>, value: int) returns (index: int)
-  requires sorted(a)
-  ensures 0 <= index ==> index < a.Length && a[index] == value
-  ensures index < 0 ==> forall k :: 0 <= k < a.Length ==> a[k] != value
-{
-    var low, high := 0, a.Length;
-    while low < high
-      invariant 0 <= low <= high <= a.Length
-      invariant forall i :: 0 <= i < a.Length && !(low <= i < high) ==> a[i] != value
-    {
-        var mid := (low + high) / 2;
-        if a[mid] < value
-        {
-            low := mid + 1;
-        }
-        else if value < a[mid]
-        {
-            high := mid;
-        }
-        else
-        {
-            return mid;
-        }
-    }
-    return -1;
-}
-
-method Main()
-{
-  var numeros := new int[5];
-  numeros[0] := 1;
-  numeros[1] := 3;
-  numeros[2] := 4;
-  numeros[3] := 6;
-  numeros[4] := 7;
-  var resultado := BinarySearch(numeros,1);
-  assert numeros[0] == 1;
-  assert resultado >= 0;
-  assert numeros[resultado] == 1;
+  var n := 0;
+  while n != a.Length
+    invariant 0 <= n <= a.Length
+    invariant forall i :: 0 <= i < n ==> a[i] == old(a[i])+1
+    invariant forall i :: n <= i < a.Length ==> a[i] == old(a[i])
+  {
+    a[n] := a[n] + 1;
+    n := n + 1;
+  }
 }
